\begin{equation}
    J = \sum_{i=1}^{n_p} \left\| Q \left( y(k+i) - y_R(k+i) \right) \right\|^2 + r \cdot \sum_{i=1}^{n_p} \left\| u(k+i-1) \right\|^2
\end{equation}

\begin{align}
    x(k+1)  &= f(x(k), u(k)) \\
    y(k)    &= g(x(k), u(k))
\end{align}

\begin{equation}
    \begin{aligned}
    C(x(t_k), s(t_k), u(\cdot), v_s(\cdot)) &= \int_{t_k}^{t_k + T_p} \left\| 
    \begin{pmatrix}
    e(\tau) \\
    a_{\text{lat}}(\tau)
    \end{pmatrix}
    \right\|_Q^2 + \left\| 
    \begin{pmatrix}
    u(\tau) \\
    v_s(\tau) - v_{s, \text{des}}(\tau)
    \end{pmatrix}
    \right\|_R^2 \, d\tau \\
    &\quad + \left\| 
    \begin{pmatrix}
    e(t_k + T_p) \\
    a_{\text{lat}}(t_k + T_p)
    \end{pmatrix}
    \right\|_P^2
    \end{aligned}
\end{equation}

\begin{equation}
    J(x(t_k),\theta(t_k),\bar{u},\bar{\vartheta}(\cdot)) = \int_{t_k}^{t_k + T_p} F(\bar{e}(\tau),\bar{x}(\tau),\bar{u}(\tau),\bar{\vartheta}(\tau))d\tau + E(\bar{e}(t_k+T_p),\bar{x}(t_k+T_p))
\end{equation}